doc-src/TutorialI/Datatype/Fundata.thy
@@ -1,7 +1,7 @@
 (*<*)
 theory Fundata = Main:
 (*>*)
-datatype ('a,'i)bigtree = Tip | Branch 'a "'i \\<Rightarrow> ('a,'i)bigtree"
+datatype ('a,'i)bigtree = Tip | Branch 'a "'i \<Rightarrow> ('a,'i)bigtree"
 
 text{*\noindent
 Parameter @{typ"'a"} is the type of values stored in
@@ -19,10 +19,10 @@ has merely @{term"Tip"}s as further subtrees.
 Function @{term"map_bt"} applies a function to all labels in a @{text"bigtree"}:
 *}
 
-consts map_bt :: "('a \\<Rightarrow> 'b) \\<Rightarrow> ('a,'i)bigtree \\<Rightarrow> ('b,'i)bigtree"
+consts map_bt :: "('a \<Rightarrow> 'b) \<Rightarrow> ('a,'i)bigtree \<Rightarrow> ('b,'i)bigtree"
 primrec
 "map_bt f Tip          = Tip"
-"map_bt f (Branch a F) = Branch (f a) (\\<lambda>i. map_bt f (F i))"
+"map_bt f (Branch a F) = Branch (f a) (\<lambda>i. map_bt f (F i))"
 
 text{*\noindent This is a valid \isacommand{primrec} definition because the
 recursive calls of @{term"map_bt"} involve only subtrees obtained from
@@ -35,16 +35,18 @@ Isabelle because the termination proof is not as obvious since
 The following lemma has a canonical proof  *}
 
 lemma "map_bt (g o f) T = map_bt g (map_bt f T)";
-by(induct_tac "T", simp_all)
+by(induct_tac T, simp_all)
 
 text{*\noindent
+%apply(induct_tac T);
+%pr(latex xsymbols symbols)
 but it is worth taking a look at the proof state after the induction step
 to understand what the presence of the function type entails:
 \begin{isabelle}
-~1.~map\_bt~g~(map\_bt~f~Tip)~=~map\_bt~(g~{\isasymcirc}~f)~Tip\isanewline
-~2.~{\isasymAnd}a~F.\isanewline
-~~~~~~{\isasymforall}x.~map\_bt~g~(map\_bt~f~(F~x))~=~map\_bt~(g~{\isasymcirc}~f)~(F~x)~{\isasymLongrightarrow}\isanewline
-~~~~~~map\_bt~g~(map\_bt~f~(Branch~a~F))~=~map\_bt~(g~{\isasymcirc}~f)~(Branch~a~F)%
+\ \isadigit{1}{\isachardot}\ map{\isacharunderscore}bt\ {\isacharparenleft}g\ {\isasymcirc}\ f{\isacharparenright}\ Tip\ {\isacharequal}\ map{\isacharunderscore}bt\ g\ {\isacharparenleft}map{\isacharunderscore}bt\ f\ Tip{\isacharparenright}\isanewline
+\ \isadigit{2}{\isachardot}\ {\isasymAnd}a\ F{\isachardot}\isanewline
+\ \ \ \ \ \ \ {\isasymforall}x{\isachardot}\ map{\isacharunderscore}bt\ {\isacharparenleft}g\ {\isasymcirc}\ f{\isacharparenright}\ {\isacharparenleft}F\ x{\isacharparenright}\ {\isacharequal}\ map{\isacharunderscore}bt\ g\ {\isacharparenleft}map{\isacharunderscore}bt\ f\ {\isacharparenleft}F\ x{\isacharparenright}{\isacharparenright}\ {\isasymLongrightarrow}\isanewline
+\ \ \ \ \ \ \ map{\isacharunderscore}bt\ {\isacharparenleft}g\ {\isasymcirc}\ f{\isacharparenright}\ {\isacharparenleft}Branch\ a\ F{\isacharparenright}\ {\isacharequal}\ map{\isacharunderscore}bt\ g\ {\isacharparenleft}map{\isacharunderscore}bt\ f\ {\isacharparenleft}Branch\ a\ F{\isacharparenright}{\isacharparenright}
 \end{isabelle}
 *}
 (*<*)
