doc-src/TutorialI/Misc/types.thy
@@ -1,8 +1,8 @@
 (*<*)
 theory "types" = Main:;
 (*>*)types number       = nat
-      gate         = "bool \\<Rightarrow> bool \\<Rightarrow> bool"
-      ('a,'b)alist = "('a * 'b)list";
+      gate         = "bool \<Rightarrow> bool \<Rightarrow> bool"
+      ('a,'b)alist = "('a \<times> 'b)list";
 
 text{*\noindent\indexbold{*types}%
 Internally all synonyms are fully expanded.  As a consequence Isabelle's
@@ -23,8 +23,8 @@ The above constants @{term"nand"} and @{term"exor"} are non-recursive and can
 therefore be defined directly by
 *}
 
-defs nand_def: "nand A B \\<equiv> \\<not>(A \\<and> B)"
-     exor_def: "exor A B \\<equiv> A \\<and> \\<not>B \\<or> \\<not>A \\<and> B";
+defs nand_def: "nand A B \<equiv> \<not>(A \<and> B)"
+     exor_def: "exor A B \<equiv> A \<and> \<not>B \<or> \<not>A \<and> B";
 
 text{*\noindent%
 where \isacommand{defs}\indexbold{*defs} is a keyword and
@@ -35,9 +35,9 @@ Declarations and definitions can also be merged
 *}
 
 constdefs nor :: gate
-         "nor A B \\<equiv> \\<not>(A \\<or> B)"
+         "nor A B \<equiv> \<not>(A \<or> B)"
           exor2 :: gate
-         "exor2 A B \\<equiv> (A \\<or> B) \\<and> (\\<not>A \\<or> \\<not>B)";
+         "exor2 A B \<equiv> (A \<or> B) \<and> (\<not>A \<or> \<not>B)";
 
 text{*\noindent\indexbold{*constdefs}%
 in which case the default name of each definition is $f$@{text"_def"}, where
