doc-src/TutorialI/Recdef/Nested1.thy
@@ -23,9 +23,9 @@ Remember that function @{term"size"} is defined for each \isacommand{datatype}.
 However, the definition does not succeed. Isabelle complains about an
 unproved termination condition
 @{term[display]"t : set ts --> size t < Suc (term_list_size ts)"}
-where @{term"set"} returns the set of elements of a list (no special
-knowledge of sets is required in the following) and @{text"term_list_size ::
-term list \<Rightarrow> nat"} is an auxiliary function automatically defined by Isabelle
+where @{term"set"} returns the set of elements of a list
+and @{text"term_list_size :: term list \<Rightarrow> nat"} is an auxiliary
+function automatically defined by Isabelle
 (when @{text"term"} was defined).  First we have to understand why the
 recursive call of @{term"trev"} underneath @{term"map"} leads to the above
 condition. The reason is that \isacommand{recdef} ``knows'' that @{term"map"}
